semantics/proofs/fpSemPropsScript.sml
@@ -2,7 +2,7 @@
   Properties of floating-point value tree semantics
 *)
 
-open preamble fpSemTheory fpValTreeTheory semanticPrimitivesTheory evaluateTheory;
+open preamble fpSemTheory fpOptPropsTheory fpValTreeTheory semanticPrimitivesTheory evaluateTheory;
 open terminationTheory;
 
 val _ = new_theory "fpSemProps";
@@ -309,9 +309,10 @@ QED
 
   local
     val eval_fp_opt_add_bind = hd (CONJ_LIST 2 (SIMP_RULE std_ss [] evaluate_fp_opt_add_bind));
+    val eval_match_fp_opt_add_bind = hd (tl (CONJ_LIST 2 (SIMP_RULE std_ss [] evaluate_fp_opt_add_bind)));
   in
 Theorem evaluate_fp_opt_add_bind_preserving:
-  ! (st1 st2:'a state) env fps1 fps2 xs r k h.
+  (! (st1 st2:'a state) env xs r k h.
     evaluate st1 env xs = (st2, r) /\
     st2.fp_state.choices <= k + st1.fp_state.choices /\
     (! m. m < k ==> h m = st1.fp_state.opts m) ==>
@@ -319,14 +320,27 @@ Theorem evaluate_fp_opt_add_bind_preserving:
       evaluate (st1 with fp_state := (st1.fp_state with opts := h)) env xs =
         (st2 with fp_state := (st2.fp_state with opts := hN), r) /\
       (! m. m < (k - (st2.fp_state.choices - st1.fp_state.choices)) ==> hN m = st2.fp_state.opts m) /\
+      (hN (k - (st2.fp_state.choices - st1.fp_state.choices)) = h k))
+  /\
+  ! (st1 st2:'a state) env v pl err_v xs r k h.
+    evaluate_match st1 env v pl err_v = (st2, r) /\
+    st2.fp_state.choices <= k + st1.fp_state.choices /\
+    (! m. m < k ==> h m = st1.fp_state.opts m) ==>
+    ? hN.
+      evaluate_match (st1 with fp_state := (st1.fp_state with opts := h)) env v pl err_v =
+        (st2 with fp_state := (st2.fp_state with opts := hN), r) /\
+      (! m. m < (k - (st2.fp_state.choices - st1.fp_state.choices)) ==> hN m = st2.fp_state.opts m) /\
       (hN (k - (st2.fp_state.choices - st1.fp_state.choices)) = h k)
 Proof
   rpt strip_tac
-  \\ first_assum (mp_then Any assume_tac eval_fp_opt_add_bind)
+  THENL [first_assum (mp_then Any assume_tac eval_fp_opt_add_bind),
+         first_assum (mp_then Any assume_tac eval_match_fp_opt_add_bind)]
   \\ pop_assum (fn asm => last_assum (mp_then Any assume_tac asm)) \\ fs[]
   \\ res_tac \\ fs[state_component_equality, fpState_component_equality]
-  \\ first_assum (mp_then Any assume_tac eval_fp_opt_inv)
-  \\ last_assum (mp_then Any assume_tac eval_fp_opt_inv)
+  \\ (first_assum (mp_then Any assume_tac eval_fp_opt_inv) ORELSE
+      first_assum (mp_then Any assume_tac evalmatch_fp_opt_inv))
+  \\ (last_assum (mp_then Any assume_tac eval_fp_opt_inv) ORELSE
+      last_assum (mp_then Any assume_tac evalmatch_fp_opt_inv))
   \\ fs[] \\ conj_tac \\ rpt strip_tac
   \\ rpt (qpat_x_assum `! x. _ = _` (fn thm => fs[GSYM thm]))
 QED
@@ -338,21 +352,207 @@ Definition optUntil_def:
 End
 
 Theorem optUntil_evaluate_ok:
-  ! st1 st2 env exps r g.
+  (! st1 st2 env exps r g.
     evaluate st1 env exps = (st2, r) ==>
     ? fpOpt.
       evaluate (st1 with fp_state := st1.fp_state with opts := optUntil (st2.fp_state.choices-st1.fp_state.choices) st1.fp_state.opts g) env exps =
-        (st2 with fp_state := (st2.fp_state with opts := g), r)
+        (st2 with fp_state := (st2.fp_state with opts := g), r)) /\
+  (! st1 st2 env v pl err_v r g.
+    evaluate_match st1 env v pl err_v = (st2, r) ==>
+    ? fpOpt.
+      evaluate_match (st1 with fp_state := st1.fp_state with opts := optUntil (st2.fp_state.choices-st1.fp_state.choices) st1.fp_state.opts g) env v pl err_v =
+        (st2 with fp_state := (st2.fp_state with opts := g), r))
 Proof
   rpt strip_tac \\ imp_res_tac evaluate_fp_opt_add_bind_preserving
   \\ first_x_assum (qspecl_then [`st2.fp_state.choices - st1.fp_state.choices `, `optUntil (st2.fp_state.choices - st1.fp_state.choices) st1.fp_state.opts g`] impl_subgoal_tac)
-  >-  (rpt strip_tac \\ fs[optUntil_def])
+  \\ TRY (fs[optUntil_def] \\ NO_TAC)
   \\ pop_assum impl_subgoal_tac \\ fs[state_component_equality, fpState_component_equality]
   \\ imp_res_tac evaluate_fp_opts_inv
   \\ rewrite_tac [FUN_EQ_THM]
   \\ fs[]
   \\ rpt (qpat_x_assum `! x. _ x = _ x` (fn thm => rewrite_tac[GSYM thm]))
   \\ fs[optUntil_def]
+QED
+
+(**
+  Next, we prove that it is always fine to append optimization by changing the
+  oracle. We cannot use the same oracle as before.
+  This is because do_fprw accesses the rewrites from the state when executing
+  the schedule. If the previous schedule failed because the rewriter was not in
+  the list, the new execution must do the same to be semantics preserving.
+  Theorem do_fprw_append_opt in fpOptPropsTheory is critical for this proof.
+**)
+local
+  val eval_goal =
+    ``\ (st1:'a semanticPrimitives$state) env el.
+        ! res st2 opts.
+          evaluate st1 env el = (st2, res) /\
+          set (st1.fp_state.rws) SUBSET set (opts) ==>
+          ? fpOpt fpOpt2.
+          evaluate (st1 with fp_state := st1.fp_state with <| rws := opts; opts := fpOpt |>) env el =
+            (st2 with fp_state := st2.fp_state with <| rws := opts; opts := fpOpt2 |>, res)``
+  val eval_match_goal =
+    ``\ (st1:'a semanticPrimitives$state) env v pl err_v.
+        ! res st2 opts.
+          evaluate_match st1 env v pl err_v = (st2, res) /\
+          set (st1.fp_state.rws) SUBSET set (opts) ==>
+          ? fpOpt fpOpt2.
+          evaluate_match (st1 with fp_state := st1.fp_state with <| rws := opts; opts := fpOpt |>) env v pl err_v =
+            (st2 with fp_state := st2.fp_state with <| rws := opts; opts := fpOpt2|>, res)``
+  val indThm = terminationTheory.evaluate_ind
+    |> ISPEC eval_goal |> SPEC eval_match_goal
+  val eval_step =  ntac 2 (reverse TOP_CASE_TAC \\ fs[]);
+  val semState_comp_eq = semanticPrimitivesTheory.state_component_equality;
+  val solve_simple =
+    rpt strip_tac \\ rveq \\ fs[] \\ first_x_assum (qspec_then `opts` impl_subgoal_tac) \\ fs[]
+    \\ qexists_tac `fpOpt` \\ qexists_tac `fpOpt2` \\ fs[];
+  val solve_complex =
+    rpt (last_x_assum (qspec_then `opts` impl_subgoal_tac))
+    \\ TRY (imp_res_tac evaluate_fp_opts_inv \\ fs[fpState_component_equality] \\ NO_TAC)
+    \\ rpt (qpat_x_assum `evaluate _ _ _ = _` kall_tac ORELSE
+            qpat_x_assum `evaluate_match _ _ _ _ _ = _` kall_tac) \\ fs[]
+    \\ (rename [`evaluate (st1 with fp_state := st1.fp_state with <| rws := _; opts := fpOpt1N |>) env [e1] =
+                  (st2 with fp_state := st2.fp_state with <| rws := _; opts := _ |>, _)`,
+                `evaluate (st2 with fp_state := st2.fp_state with <| rws := _; opts := fpOpt2N |>) _ _ =
+                  (st3 with fp_state := st3.fp_state with <| rws := _; opts := fpOpt3N |>, _)`]
+        ORELSE
+      rename [`evaluate (st1 with fp_state := st1.fp_state with <| rws := _; opts := fpOpt1N |>) env [e1] =
+                  (st2 with fp_state := st2.fp_state with <| rws := _; opts := _ |>, _)`,
+               `evaluate_match (st2 with fp_state := st2.fp_state with <| rws := _; opts := fpOpt2N |>) env _ _ _=
+                  (st3 with fp_state := st3.fp_state with <| rws := _; opts := fpOpt3N |>, _)`]
+      ORELSE
+      rename [`evaluate (st1 with fp_state := st1.fp_state with <| rws := _; opts := fpOpt1N |>) env (REVERSE es) =
+                  (st2 with fp_state := st2.fp_state with <| rws := _; opts := _ |>, _)`,
+               `evaluate (st2 with <| clock := st2.clock - 1; fp_state := st2.fp_state with <| rws := _; opts := fpOpt2N |> |>) _ _ =
+                  (st3 with fp_state := st3.fp_state with <| rws := _; opts := fpOpt3N|>, _)`])
+    \\ qexists_tac `optUntil (st2.fp_state.choices - st1.fp_state.choices) fpOpt1N fpOpt2N`
+    \\ rpt (first_x_assum (fn thm => (mp_then Any assume_tac (CONJUNCT1 optUntil_evaluate_ok) thm) \\ mp_tac thm))
+    \\ rpt (first_x_assum (qspec_then `fpOpt2N` assume_tac))
+    \\ fs[fpState_component_equality, semState_comp_eq];
+in
+Theorem evaluate_fp_rws_up:
+  (! (st1:'a semanticPrimitives$state) env el.
+    ^eval_goal st1 env el) /\
+  (! (st1:'a semanticPrimitives$state) env v pl err_v.
+    ^eval_match_goal st1 env v pl err_v)
+Proof
+  match_mp_tac indThm
+  \\ rpt strip_tac \\ fs[evaluate_def] \\ rpt strip_tac \\ rveq \\ fs[fpState_component_equality]
+  \\ TRY (qexists_tac `\ x. []` \\ fs[fpState_component_equality, semState_comp_eq] \\ NO_TAC)
+  \\ qpat_x_assum `_ = (_, _)` mp_tac
+  (* e1 :: e2 :: es *)
+  >- (
+    eval_step >- solve_simple
+    \\ ntac 2 (TOP_CASE_TAC)
+    \\ rpt strip_tac \\ rveq \\ fs[]
+    \\ solve_complex)
+  (* Raise e *)
+  >- (eval_step \\ solve_simple)
+  (* match *)
+  >- (
+    ntac 2 (TOP_CASE_TAC \\ fs[]) >- solve_simple
+    \\ reverse TOP_CASE_TAC \\ fs[] >- solve_simple
+    \\ rpt strip_tac \\ fs[]
+    \\ solve_complex)
+  (* do_con_check *)
+  >- (
+      reverse TOP_CASE_TAC \\ fs[]
+      >- (rpt strip_tac \\ rveq \\ fs[fpState_component_equality, semState_comp_eq])
+      \\ eval_step >- solve_simple
+      \\ TOP_CASE_TAC \\ solve_simple)
+  (* Variable lookup *)
+  >- (TOP_CASE_TAC \\ fs[fpState_component_equality, semState_comp_eq])
+  (* do_app *)
+  >- (
+    eval_step >- solve_simple
+    \\ TOP_CASE_TAC \\ fs[]
+    >- (TOP_CASE_TAC \\ fs[] >- solve_simple
+        \\ ntac 2 (TOP_CASE_TAC \\ fs[]) >- solve_simple
+        \\ strip_tac \\ fs[dec_clock_def]
+        \\ solve_complex)
+    \\ TOP_CASE_TAC \\ fs[] >- solve_simple
+    \\ ntac 3 (reverse TOP_CASE_TAC \\ fs[]) >- solve_simple
+    \\ rename [`evaluate st1 env (REVERSE es) = (st2,Rval res)`]
+    \\ `set st2.fp_state.rws SUBSET set opts`
+        by (imp_res_tac evaluate_fp_opts_inv \\ fs[fpState_component_equality])
+    \\ qpat_x_assum `evaluate _ _ _ = _` kall_tac
+    \\ first_x_assum (qspec_then `opts` impl_subgoal_tac) \\ fs[]
+    \\ rename [`evaluate (st1 with fp_state := st1.fp_state with <| rws := opts; opts := fpOpt1 |>) env (REVERSE es) =
+                  (st2 with fp_state := _, _)`]
+    \\ Cases_on `st2.fp_state.canOpt` \\ fs[]
+    >- (rpt strip_tac \\ rveq
+        \\ fs[shift_fp_opts_def, fpState_component_equality]
+        \\ first_x_assum (mp_then Any assume_tac (CONJUNCT1 optUntil_evaluate_ok))
+        \\ Cases_on `do_fprw r (st2.fp_state.opts 0) st2.fp_state.rws`
+        \\ imp_res_tac do_fprw_up
+        \\ first_x_assum (qspec_then `\x. sched2` assume_tac)
+        \\ qexists_tac `optUntil (st2.fp_state.choices - st1.fp_state.choices) fpOpt1 (\x. sched2)`
+        \\ fs[fpState_component_equality, semState_comp_eq])
+    \\ rpt strip_tac \\ rveq
+    \\ qexists_tac `fpOpt1` \\ fs[fpState_component_equality, semState_comp_eq])
+  (* Log_op *)
+  >- (
+    eval_step >- solve_simple
+    \\ TOP_CASE_TAC \\ fs[] >- solve_simple
+    \\ reverse TOP_CASE_TAC \\ fs[] >- solve_simple
+    \\ rpt strip_tac \\ fs[]
+    \\ solve_complex)
+  (* do_if *)
+  >- (
+    eval_step >- solve_simple
+    \\ TOP_CASE_TAC \\ fs[] >- solve_simple
+    \\ rpt strip_tac \\ fs[]
+    \\ solve_complex)
+  (* match bind_exn_v *)
+  >- (
+    eval_step >- solve_simple
+    \\ rpt strip_tac \\ fs[]
+    \\ solve_complex)
+  (* let binding *)
+  >- (
+    eval_step >- solve_simple
+    \\ rpt strip_tac \\ fs[]
+    \\ solve_complex)
+  (* ALL_DISTINCT *)
+  >- (
+    reverse TOP_CASE_TAC >- fs[fpState_component_equality, semState_comp_eq]
+    \\ strip_tac \\ fs[])
+  (* FpOptimise *)
+  >- (
+    ntac 2 (reverse TOP_CASE_TAC \\ fs[]) >- solve_simple
+    \\ rpt strip_tac \\ fs[] \\ rveq
+    \\ first_x_assum (qspec_then `opts` impl_subgoal_tac)
+    \\ fs[] \\ qexists_tac `fpOpt` \\ qexists_tac `fpOpt2`
+    \\ fs[])
+  (* ALL_DISTINCT (pat_bindings) *)
+  >- (
+    rpt (reverse TOP_CASE_TAC \\ fs[fpState_component_equality, semState_comp_eq]))
+QED
+end
+
+Theorem evaluate_fp_rws_append:
+  (! (st1:'a semanticPrimitives$state) env el res st2 opts.
+    evaluate st1 env el = (st2, res) ==>
+    ! g.
+    ? fpOpt.
+    evaluate (st1 with fp_state := st1.fp_state with <| rws := st1.fp_state.rws ++ opts; opts := fpOpt |>) env el =
+      (st2 with fp_state := st2.fp_state with <| rws := st2.fp_state.rws ++ opts; opts := g |>, res)) /\
+  ! (st1:'a semanticPrimitives$state) env v pl err_v res st2 opts.
+    evaluate_match st1 env v pl err_v = (st2, res) ==>
+    ! g.
+    ? fpOpt.
+    evaluate_match (st1 with fp_state := st1.fp_state with <| rws := st1.fp_state.rws ++ opts; opts := fpOpt |>) env v pl err_v =
+      (st2 with fp_state := st2.fp_state with <| rws := st2.fp_state.rws ++ opts; opts := g |>, res)
+Proof
+  rpt strip_tac \\ imp_res_tac (SIMP_RULE std_ss [] evaluate_fp_rws_up)
+  \\ first_x_assum (qspec_then `st1.fp_state.rws ++ opts` impl_subgoal_tac) \\ fs[]
+  THENL [first_x_assum (mp_then Any assume_tac (CONJUNCT1 optUntil_evaluate_ok)),
+         first_x_assum (mp_then Any assume_tac (CONJUNCT2 optUntil_evaluate_ok))]
+  \\ first_x_assum (qspec_then `g` assume_tac) \\ fs[]
+  \\ `st1.fp_state.rws = st2.fp_state.rws` by (imp_res_tac evaluate_fp_opts_inv \\ fs[])
+  \\ fs[]
+  \\ asm_exists_tac
+  \\ fs[fpState_component_equality, state_component_equality]
 QED
 
 (** UNUSED STUFF BEGINS HERE
